Add a dynamic store initialization function to the monadic translator

translator/monadic/ml_monadStoreLib.sig
@@ -4,23 +4,25 @@ sig
     type term = Term.term
     type hol_type = Type.hol_type
 
+    type monadic_translation_parameters =
+    {store_pred_def : thm,
+     refs_specs : (thm * thm) list,
+     arrays_specs : (thm * thm * thm * thm) list};
+
     type store_translation_result =
     {refs_init_values : thm list,
      refs_locations  : thm list,
      arrays_init_values : thm list,
      arrays_locations : thm list,
-     store_pred_def : thm,
      store_pred_validity : thm,
-     store_pred_exists_thm : thm,
-     refs_specs : (thm * thm) list,
-     arrays_specs : (thm * thm * thm * thm) list};
+     store_pred_exists_thm : thm};
 
-   val mk_store_translation_result :
-       thm list -> thm list -> thm list -> thm list -> thm -> thm -> thm -> (thm * thm) list ->
-       (thm * thm * thm * thm) list -> store_translation_result
+  val translate_dynamic_init_fixed_store  : (string * thm * thm) list ->
+       (string * thm * thm * thm * thm * thm * thm) list ->
+       string -> hol_type -> thm -> monadic_translation_parameters
 
-   val translate_fixed_store :
+   val translate_static_init_fixed_store :
        (string * thm * thm * thm) list ->
        (string * thm * thm * thm * thm * thm * thm * thm) list ->
-       string -> hol_type -> thm -> store_translation_result
+       string -> hol_type -> thm -> monadic_translation_parameters * store_translation_result
 end
